src/ByteStringCanon.v
@@ -202,21 +202,27 @@ Proof.
   start sharpening ADT.
 
   hone representation using
-       (fun or nr => Heap_AbsR (fst or) (fst nr) /\ snd or = snd nr).
+       (fun (or : bsrep) (nr : Comp (cHeapRep * PS)) =>
+          exists oh ops nh nps,
+            or ↝ (oh, ops) /\
+            nr ↝ (nh, nps) /\
+            Heap_AbsR oh nh /\ ops = nps).
 
   (* refine method ByteString.emptyS. *)
   {
     simplify with monad laws.
-    refine pick val (heap', {| psBuffer := 0
-                             ; psBufLen := 0
-                             ; psOffset := 0
-                             ; psLength := 0 |}).
+    refine pick val (ret (heap', {| psBuffer := 0
+                                  ; psBufLen := 0
+                                  ; psOffset := 0
+                                  ; psLength := 0 |})).
       finish honing.
-    firstorder.
+    do 4 eexists; split; eauto.
   }
 
   (* refine method ByteString.consS. *)
   {
+    admit.
+(*
     apply_ByteString_Heap_AbsR.
     fracture H; unfold find_free_block;
     refine using ByteString_Heap_AbsR;
@@ -259,10 +265,13 @@ Proof.
     - rewrite resvs_match0.
       eapply for_all_impl; eauto;
       relational; nomega.
+*)
   }
 
   (* refine method ByteString.unconsS. *)
   {
+    admit.
+(*
     unfold buffer_uncons;
     apply_ByteString_Heap_AbsR;
     fracture H;
@@ -294,12 +303,15 @@ Proof.
         finish honing.
       split; trivial.
       constructor; auto.
+*)
   }
 
   (* refine method ByteString.appendS. *)
   {
     unfold buffer_append, alloc, Bind2, find_free_block; simpl.
 
+    admit.
+(*
     rewrite !refine_IfDep_Then_Else_Bind,
             !refineEquiv_strip_IfDep_Then_Else.
     refine pick val (plusPtr (A:=Word) (fst (fst r_n)) 1).
@@ -378,6 +390,7 @@ Proof.
     remember (fun _ _ => _) as P.
     remember (fun _ _ => negb _) as P'.
     apply for_all_impl with (P:=P) (P':=P'); relational; nomega.
+*)
   }
 
   (** Apply some common functional optimizations, such as common subexpression
@@ -406,9 +419,12 @@ Proof.
     simplify with monad laws.
     refine pick eq.
     simplify with monad laws.
+    admit.
+(*
     rewrite !If_Then_Else_fst, !If_Then_Else_snd; simpl.
     rewrite If_Then_Else_pair.
     subst; finish honing.
+*)
   }
 
   (* refine method ByteString.appendS. *)
@@ -418,7 +434,8 @@ Proof.
   }
 
   finish_SharpeningADT_WithoutDelegation.
-Defined.
+Admitted.
+(* Defined. *)
 
 End Refined.
 
